[WIP] Change sim_memory to have same cover of half messages

src/opt/SimMemory.v
@@ -42,6 +42,31 @@ Next Obligation.
   ii. inv H; inv H0; econs. etrans; eauto.
 Qed.
 
+Inductive same_message_kind: forall (msg_src msg_tgt: Message.t), Prop :=
+| same_message_kind_full
+    val_src val_tgt released_src released_tgt:
+    same_message_kind (Message.mk val_src released_src) (Message.mk val_tgt released_tgt)
+| same_message_kine_half:
+    same_message_kind Message.half Message.half
+.
+Hint Constructors sim_message.
+
+Program Instance same_message_kind_PreOrder: PreOrder same_message_kind.
+Next Obligation.
+  ii. destruct x; econs.
+Qed.
+Next Obligation.
+  ii. inv H; inv H0; econs.
+Qed.
+
+Lemma sim_message_same_message_kind
+      msg_src msg_tgt
+      (SIM: sim_message msg_src msg_tgt):
+  same_message_kind msg_src msg_tgt.
+Proof.
+  inv SIM; econs.
+Qed.
+
 Inductive covered (loc:Loc.t) (ts:Time.t) (mem:Memory.t): Prop :=
 | covered_intro
     from to msg
@@ -90,54 +115,213 @@ Proof.
   eapply SIM. eauto.
 Qed.
 
-(* Lemma sim_memory_max_timemap *)
-(*       mem_src mem_tgt mtm_src mtm_tgt *)
-(*       (CLOSED_SRC: Memory.closed mem_src) *)
-(*       (CLOSED_TGT: Memory.closed mem_tgt) *)
+Lemma sim_memory_get_from
+      loc from_src from_tgt to_src to_tgt msg_src msg_tgt mem_src mem_tgt
+      (SIM: sim_memory mem_src mem_tgt)
+      (GET_SRC: Memory.get loc to_src mem_src = Some (from_src, msg_src))
+      (GET_TGT: Memory.get loc to_tgt mem_tgt = Some (from_tgt, msg_tgt))
+      (FROM: Time.lt from_tgt from_src)
+      (TO: Time.le to_src to_tgt):
+  exists from_src' msg_src',
+    Memory.get loc from_src mem_src = Some (from_src', msg_src').
+Proof.
+  exploit Memory.get_ts; try exact GET_SRC. i.
+  exploit Memory.get_ts; try exact GET_TGT. i.
+  des; subst; try by inv FROM.
+  { subst. inv TO; inv H. inv x0. }
+  inv SIM. specialize (COVER loc from_src). des.
+  exploit COVER0.
+  { econs; eauto. econs; timetac.
+    econs. eapply TimeFacts.lt_le_lt; eauto. }
+  i. inv x.
+  destruct (Time.eq_dec to from_src).
+  { subst. esplits; eauto. }
+  inv ITV. ss. inv TO0; cycle 1.
+  { inv H. congr. }
+  exploit MemoryFacts.get_disjoint; [exact GET_SRC|exact GET|..]. i. des.
+  { subst. timetac. }
+  exfalso. destruct (Time.le_lt_dec to_src to).
+  - apply (x2 to_src).
+    + econs; eauto. refl.
+    + econs; eauto.
+  - apply (x2 to).
+    + repeat econs; eauto.
+    + econs; eauto. refl.
+Qed.
+
+Lemma sim_memory_get_inv
+      loc from_src to_src msg_src mem_src
+      mem_tgt
+      (INHABITED_SRC: Memory.inhabited mem_src)
+      (INHABITED_TGT: Memory.inhabited mem_tgt)
+      (SIM: sim_memory mem_src mem_tgt)
+      (GET_SRC: Memory.get loc to_src mem_src = Some (from_src, msg_src)):
+  exists from_tgt to_tgt msg_tgt,
+    <<FROM: Time.le from_tgt from_src>> /\
+    <<TO: Time.le to_src to_tgt>> /\
+    <<GET_TGT: Memory.get loc to_tgt mem_tgt = Some (from_tgt, msg_tgt)>> /\
+    <<MSG: same_message_kind msg_src msg_tgt>>.
+Proof.
+  destruct (Time.eq_dec to_src Time.bot).
+  { subst. rewrite INHABITED_SRC in GET_SRC. inv GET_SRC.
+    esplits; try refl. apply INHABITED_TGT. }
+  inv SIM. dup COVER. specialize (COVER0 loc to_src). des.
+  exploit COVER0.
+  { econs; eauto. econs; try refl.
+    exploit Memory.get_ts; eauto. i. des; subst; timetac. }
+  i. dup x. inv x0. esplits; eauto.
+  - destruct (Time.le_lt_dec from from_src); ss.
+    dup COVER. specialize (COVER2 loc from). des. exploit COVER2.
+    { econs; eauto.
+      exploit Memory.get_ts; try exact GET_SRC. i. des; ss.
+      inv ITV. econs; eauto. econs. ss. }
+    i. inv x0.
+    destruct (Time.eq_dec to0 from).
+    + subst. exploit MSG; try exact GET0. i. des.
+      exploit MemoryFacts.get_disjoint; [exact GET_SRC|exact GET1|..]. i. des.
+      * subst. inv ITV. timetac.
+      * exfalso. apply (x1 from).
+        { inv ITV. econs; eauto. s. econs; eauto. }
+        { econs; try refl. s.
+          exploit Memory.get_ts; try exact GET1. i. des; ss.
+          subst. inv ITV0. inv FROM. }
+    + exploit MemoryFacts.get_disjoint; [exact GET|exact GET0|..]. i. des.
+      * subst. inv ITV0. timetac.
+      * exfalso. destruct (Time.le_lt_dec to to0).
+        { apply (x1 to).
+          - econs; try refl.
+            exploit Memory.get_ts; try exact GET. i. des; ss.
+            subst. inv ITV0. inv FROM.
+          - econs; eauto. inv ITV0. ss.
+            exploit Memory.get_ts; try exact GET. i. des; ss.
+            + subst. inv l.
+            + eapply TimeFacts.lt_le_lt; eauto. econs; eauto. }
+        { apply (x1 to0).
+          - inv ITV0. econs; ss.
+            + inv TO; ss. inv H. congr.
+            + econs. ss.
+          - econs; try refl.
+            exploit Memory.get_ts; try exact GET0. i. des; ss.
+            subst. inv ITV0. ss. inv TO; inv H. inv FROM. }
+  - inv ITV. ss.
+  - destruct msg_src; destruct msg; try econs.
+    + specialize (COVER_HALF loc to_src). des.
+      exploit COVER_HALF0; try by econs; eauto. i. inv x0.
+      destruct (Time.eq_dec to_src to0).
+      * subst. rewrite GET_SRC in GET0. inv GET0.
+      * exfalso.
+        exploit MemoryFacts.get_disjoint; [exact GET_SRC|exact GET0|..]. i. des; ss.
+        apply (x1 to_src); auto.
+        exploit Memory.get_ts; try exact GET_SRC. i.
+        exploit Memory.get_ts; try exact GET0. i. des; ss.
+        { subst. rewrite INHABITED_SRC in GET0. inv GET0. }
+        { econs; eauto. refl. }
+    + specialize (COVER_HALF loc to_src). des.
+      exploit COVER_HALF.
+      { econs; eauto.
+        exploit Memory.get_ts; try exact GET_SRC. i. des; ss.
+        econs; eauto. refl. }
+      i. inv x0.
+      destruct (Time.eq_dec to to0).
+      * subst. rewrite GET in GET0. inv GET0.
+      * exfalso.
+        exploit MemoryFacts.get_disjoint; [exact GET|exact GET0|..]. i. des; ss.
+        apply (x1 to_src); auto.
+Qed.
+
+(* Lemma sim_memory_get_from *)
+(*       loc from_src from_tgt to msg_src msg_tgt mem_src mem_tgt *)
 (*       (SIM: sim_memory mem_src mem_tgt) *)
-(*       (MAX_SRC: Memory.max_full_timemap mem_src mtm_src) *)
-(*       (MAX_TGT: Memory.max_full_timemap mem_tgt mtm_tgt): *)
-(*   mtm_src = mtm_tgt. *)
+(*       (GET_SRC: Memory.get loc to mem_src = Some (from_src, msg_src)) *)
+(*       (GET_TGT: Memory.get loc to mem_tgt = Some (from_tgt, msg_tgt)): *)
+(*   <<FROM: Time.le from_tgt from_src>> /\ *)
+(*   <<MSG: sim_message msg_src msg_tgt>>. *)
 (* Proof. *)
-(*   apply TimeMap.antisym. *)
-(*   - eapply Memory.max_full_timemap_spec'; eauto. i. *)
-(*     destruct (Time.le_lt_dec (mtm_src loc) Time.bot). *)
-(*     { esplits; eauto. apply CLOSED_TGT. } *)
-(*     exploit Memory.max_full_timemap_closed; try apply MAX_SRC; eauto. *)
-(*     instantiate (1 := loc). i. des. *)
-(*     inv SIM. destruct (COVER loc (mtm_src loc)) as [C1 C2]. *)
-(*     exploit C1; eauto. *)
-(*     { econs; eauto. apply Interval.mem_ub. *)
-(*       destruct (mem_src loc).(Cell.WF). exploit VOLUME; eauto. i. des; auto. *)
-(*       inv x. rewrite H1 in *. inv l. *)
-(*     } *)
-(*     i. inv x. inv ITV. destruct msg. ss. *)
-(*     esplits; eauto. *)
+(*   inv SIM. split; cycle 1. *)
+(*   { exploit MSG; eauto. i. des. *)
+(*     rewrite GET in GET_SRC. inv GET_SRC. ss. } *)
+(*   destruct (Time.le_lt_dec from_tgt from_src); ss. *)
+(*   generalize COVER. intro X. *)
+(*   specialize (X loc from_tgt). des. *)
+(*   exploit X. *)
+(*   { econs; eauto. econs; ss. *)
+(*     exploit Memory.get_ts; try exact GET_TGT. *)
+(*     i. des; subst. *)
+(*     - inv l. *)
+(*     - econs. ss. } *)
+(*   i. inv x. *)
+(*   exploit MemoryFacts.get_disjoint; [exact GET_TGT|exact GET|..]. *)
+(*   i. des. *)
+(*   - subst. inv ITV. ss. timetac. *)
+(*   - exploit Memory.get_ts; try exact GET_TGT. i. *)
+(*     exploit Memory.get_ts; try exact GET. i. *)
+(*     des; subst; try by apply Time.bot_spec. *)
+(*     { inv ITV. ss. timetac. } *)
+(*     destruct (Time.le_lt_dec to to0). *)
+(*     + exploit (x0 to); ss; econs; timetac; try refl. *)
+(*       inv ITV. etrans; eauto. *)
+(*     + exploit MSG; try exact GET. i. des. *)
+(*       exploit Memory.get_ts; try exact GET_SRC. i. *)
+(*       exploit Memory.get_ts; try exact GET0. i. *)
+(*       des; subst; timetac. *)
+(*       { inv x2. } *)
+(*       { inv l0. } *)
+(*       exploit MemoryFacts.get_disjoint;  [exact GET_SRC|exact GET0|..]. *)
+(*       i. des; timetac. *)
+(*       inv ITV. ss. exfalso. apply (x5 to0); econs; ss; try refl. *)
+(*       * eapply TimeFacts.lt_le_lt; try exact l. ss. *)
+(*       * econs; eauto. *)
 (* Qed. *)
 
-(* Lemma sim_memory_max_view *)
-(*       mem_src mem_tgt *)
-(*       (CLOSED_SRC: Memory.closed mem_src) *)
-(*       (CLOSED_TGT: Memory.closed mem_tgt) *)
-(*       (SIM: sim_memory mem_src mem_tgt): *)
-(*   View.le (Memory.max_view mem_src) (Memory.max_view mem_tgt). *)
-(* Proof. *)
-(*   econs; apply sim_memory_max_timemap; auto. *)
-(* Qed. *)
+Lemma sim_memory_max_full_timemap
+      mem_src mem_tgt mtm_src mtm_tgt
+      (CLOSED_SRC: Memory.closed mem_src)
+      (CLOSED_TGT: Memory.closed mem_tgt)
+      (SIM: sim_memory mem_src mem_tgt)
+      (MAX_SRC: Memory.max_full_timemap mem_src mtm_src)
+      (MAX_TGT: Memory.max_full_timemap mem_tgt mtm_tgt):
+  mtm_src = mtm_tgt.
+Proof.
+  apply TimeMap.antisym.
+  - eapply Memory.max_full_timemap_spec'; eauto. i.
+    destruct (MAX_SRC loc). des.
+    exploit sim_memory_get_inv; eauto.
+    { apply CLOSED_SRC. }
+    { apply CLOSED_TGT. }
+    i. des. inv MSG. esplits; eauto.
+  - eapply Memory.max_full_timemap_spec'; eauto. i.
+    destruct (MAX_TGT loc). des.
+    inv SIM. exploit MSG; eauto. i. des.
+    inv MSG0. esplits; eauto.
+Qed.
 
-(* Lemma sim_memory_max_released *)
-(*       mem_src mem_tgt loc ts *)
-(*       (CLOSED_SRC: Memory.closed mem_src) *)
-(*       (CLOSED_TGT: Memory.closed mem_tgt) *)
-(*       (SIM: sim_memory mem_src mem_tgt): *)
-(*   View.le (Memory.max_released mem_src loc ts) (Memory.max_released mem_tgt loc ts). *)
-(* Proof. *)
-(*   unfold Memory.max_released. econs; s. *)
-(*   - ii. unfold TimeMap.add. condtac; [refl|]. *)
-(*     eapply sim_memory_max_timemap; eauto. *)
-(*   - ii. unfold TimeMap.add. condtac; [refl|]. *)
-(*     eapply sim_memory_max_timemap; eauto. *)
-(* Qed. *)
+Lemma sim_memory_max_full_view
+      mem_src mem_tgt mview_src mview_tgt
+      (CLOSED_SRC: Memory.closed mem_src)
+      (CLOSED_TGT: Memory.closed mem_tgt)
+      (SIM: sim_memory mem_src mem_tgt)
+      (MAX_SRC: Memory.max_full_view mem_src mview_src)
+      (MAX_TGT: Memory.max_full_view mem_tgt mview_tgt):
+  mview_src = mview_tgt.
+Proof.
+  inv MAX_SRC. inv MAX_TGT.
+  exploit sim_memory_max_full_timemap; try exact SIM; eauto. i.
+  subst. ss.
+Qed.
+
+Lemma sim_memory_max_full_released
+      mem_src mem_tgt loc ts mr_src mr_tgt
+      (CLOSED_SRC: Memory.closed mem_src)
+      (CLOSED_TGT: Memory.closed mem_tgt)
+      (SIM: sim_memory mem_src mem_tgt)
+      (MAX_SRC: Memory.max_full_released mem_src loc ts mr_src)
+      (MAX_TGT: Memory.max_full_released mem_tgt loc ts mr_tgt):
+  mr_src = mr_tgt.
+Proof.
+  inv MAX_SRC. inv MAX_TGT.
+  exploit sim_memory_max_full_timemap; try exact SIM; eauto. i.
+  subst. ss.
+Qed.
 
 Lemma covered_disjoint
       mem1 mem2 loc from to
@@ -273,15 +457,14 @@ Proof.
       des; congr.
 Qed.
 
-(* Lemma split_covered_half *)
-(*       mem2 mem1 loc ts1 ts2 ts3 msg2 msg3 *)
-(*       l t *)
-(*       (SPLIT: Memory.split mem1 loc ts1 ts2 ts3 msg2 msg3 mem2): *)
-(*   covered_half l t mem2 <-> *)
-(*   (msg2 = Message.half /\ message3 = Message.half /\ covered_half l t mem1) \/ *)
-(*   (msg2 = Message.half /\ *)
-(*   (msg2 = Message.half /\ l = loc /\ Interval.mem (ts1, ts2) t). *)
-(* Proof. *)
+Lemma split_covered_half
+      mem2 mem1 loc ts1 ts2 ts3 msg2 msg3
+      l t
+      (SPLIT: Memory.split mem1 loc ts1 ts2 ts3 msg2 msg3 mem2):
+  covered_half l t mem2 <->
+  ((l <> loc \/ ~ Interval.mem (ts1, ts2) t) /\ covered_half l t mem1) \/
+  (msg2 = Message.half /\ l = loc /\ Interval.mem (ts1, ts2) t).
+Proof.
 (*   econs; i. *)
 (*   - exploit Memory.split_get0; eauto. i. des. *)
 (*     inv H. revert GET3. erewrite Memory.split_o; eauto. repeat condtac; ss. *)
@@ -315,7 +498,49 @@ Qed.
 (*       * guardH o. des. subst. congr. *)
 (*       * guardH o. guardH o0. des. subst. *)
 (*         unguardH o. des; congr. *)
-(* Qed. *)
+Admitted.
+
+Lemma split_covered_half_same
+      mem2 mem1 loc ts1 ts2 ts3 msg3
+      l t
+      (SPLIT: Memory.split mem1 loc ts1 ts2 ts3 msg3 msg3 mem2):
+  covered_half l t mem2 <-> covered_half l t mem1.
+Proof.
+  econs; i.
+  - exploit Memory.split_get0; eauto. i. des.
+    inv H. revert GET3. erewrite Memory.split_o; eauto. repeat condtac; ss.
+    + des. subst. i. inv GET3. econs; eauto.
+      eapply Interval.le_mem; eauto. econs; [refl|].
+      inv SPLIT. inv SPLIT0. left. auto.
+    + guardH o. des. subst. i. inv GET3. econs; eauto.
+      eapply Interval.le_mem; eauto. econs; [|refl].
+      inv SPLIT. inv SPLIT0. left. auto.
+    + i. econs; eauto.
+  - exploit Memory.split_get0; eauto. i. des.
+    inv H.
+    destruct (loc_ts_eq_dec (l, to) (loc, ts3)); ss.
+    + des. subst. rewrite GET0 in GET3. inv GET3.
+      destruct (Time.le_lt_dec t ts2).
+      * econs.
+        { instantiate (1 := from). instantiate (1 := ts2).
+          erewrite Memory.split_o; eauto. condtac; ss.
+          des; congr.
+        }
+        { inv ITV. econs; ss. }
+      * econs.
+        { instantiate (1 := ts2). instantiate (1 := ts3).
+          erewrite Memory.split_o; eauto. repeat condtac; ss.
+          - des. subst. inv SPLIT. inv SPLIT0.
+            exfalso. eapply Time.lt_strorder. eauto.
+          - guardH o. des; congr.
+        }
+        { inv ITV. econs; ss. }
+    + econs; eauto. erewrite Memory.split_o; eauto.
+      repeat condtac; ss; eauto.
+      * guardH o. des. subst. congr.
+      * guardH o. guardH o0. des. subst.
+        unguardH o. des; congr.
+Qed.
 
 Lemma lower_covered_half
       mem2 mem1 loc from to msg1 msg2
@@ -325,31 +550,139 @@ Lemma lower_covered_half
   ((l <> loc \/ ~ Interval.mem (from, to) t) /\ covered_half l t mem1) \/
   (l = loc /\ Interval.mem (from, to) t /\ msg2 = Message.half).
 Proof.
-  econs; i.
-  - exploit Memory.lower_get0; eauto. i. des.
-    inv H.
-    destruct (loc_ts_eq_dec (l, to0) (loc, to)); ss.
-    + des. subst. rewrite GET0 in GET1. inv GET1. eauto.
-    + left. split.
-      * des; eauto. destruct (Loc.eq_dec l loc); eauto.
-        subst. inv LOWER. unfold Memory.get in *. ss.
-        rewrite LocFun.add_spec in GET0, GET1.
-        exploit Cell.lower_wf; eauto.
-    inv H. revert GET. erewrite Memory.lower_o; eauto. condtac; ss.
-    + des. subst. i. inv GET. right. left.
-      hexploit Memory.lower_get0; eauto. i. des. inv MSG_LE.
-      esplits; eauto. econs; eauto.
-    + i. econs; eauto.
-  - exploit Memory.lower_get0; eauto. i. des.
-    inv H.
-    destruct (loc_ts_eq_dec (l, to0) (loc, to)); ss.
-    + des. subst. econs; cycle 1; eauto.
-      erewrite Memory.lower_o; eauto. condtac; [|by des].
-      rewrite GET in GET1. inv GET1. eauto.
+  (* econs; i. *)
+  (* - exploit Memory.lower_get0; eauto. i. des. *)
+  (*   inv H. *)
+  (*   destruct (loc_ts_eq_dec (l, to0) (loc, to)); ss. *)
+  (*   + des. subst. rewrite GET0 in GET1. inv GET1. eauto. *)
+  (*   + left. split. *)
+  (*     * des; eauto. destruct (Loc.eq_dec l loc); eauto. *)
+  (*       subst. inv LOWER. unfold Memory.get in *. ss. *)
+  (*       rewrite LocFun.add_spec in GET0, GET1. *)
+  (*       exploit Cell.lower_wf; eauto. *)
+  (*   inv H. revert GET. erewrite Memory.lower_o; eauto. condtac; ss. *)
+  (*   + des. subst. i. inv GET. right. left. *)
+  (*     hexploit Memory.lower_get0; eauto. i. des. inv MSG_LE. *)
+  (*     esplits; eauto. econs; eauto. *)
+  (*   + i. econs; eauto. *)
+  (* - exploit Memory.lower_get0; eauto. i. des. *)
+  (*   inv H. *)
+  (*   destruct (loc_ts_eq_dec (l, to0) (loc, to)); ss. *)
+  (*   + des. subst. econs; cycle 1; eauto. *)
+  (*     erewrite Memory.lower_o; eauto. condtac; [|by des]. *)
+  (*     rewrite GET in GET1. inv GET1. eauto. *)
+  (*   + econs; eauto. *)
+  (*     erewrite Memory.lower_o; eauto. rewrite GET1. condtac; ss. *)
+  (*     des; congr. *)
+Admitted.
+
+Lemma sim_memory_split_exists_aux
+      ts1 ts2 ts3
+      loc from_src msg_src mem_src
+      msg_tgt mem1_tgt
+      (SIM: sim_memory mem_src mem1_tgt)
+      (GET_SRC: Memory.get loc ts2 mem_src = Some (from_src, msg_src))
+      (GET_TGT: Memory.get loc ts3 mem1_tgt = Some (ts1, msg_tgt))
+      (CLOSED_SRC: Memory.closed mem_src)
+      (CLOSED_TGT: Memory.closed mem1_tgt)
+      (TS12: Time.lt ts1 ts2)
+      (TS23: Time.lt ts2 ts3):
+  exists msg_tgt' mem2_tgt,
+    <<SPLIT: Memory.split mem1_tgt loc ts1 ts2 ts3 msg_tgt' msg_tgt mem2_tgt>> /\
+    <<MSG_WF: Message.wf msg_tgt'>> /\
+    <<MSG_TS: Memory.message_ts msg_tgt' loc ts2>> /\
+    <<MSG_CLOSED: Memory.closed_message_view msg_tgt' mem2_tgt>> /\
+    <<MSG_SIM: sim_message msg_src msg_tgt'>>.
+Proof.
+  destruct msg_src.
+  - exploit (@Memory.max_full_released_exists mem1_tgt loc ts2); try apply CLOSED_TGT. i. des.
+    exploit Memory.max_full_released_wf; eauto. i.
+    exploit (@Memory.split_exists mem1_tgt loc ts1 ts2 ts3 (Message.mk val (Some released0)) msg_tgt); eauto.
+    { econs. eauto. }
+    i. des.
+    exploit Memory.max_full_released_closed_split; eauto. i. des.
+    esplits; eauto.
     + econs; eauto.
-      erewrite Memory.lower_o; eauto. rewrite GET1. condtac; ss.
-      des; congr.
+    + econs; eauto.
+      exploit (@Memory.max_full_released_exists mem_src loc ts2); try apply CLOSED_SRC. i. des.
+      exploit sim_memory_max_full_released; try exact SIM; eauto. i. subst.
+      inv CLOSED_SRC. exploit CLOSED0; eauto. i. des.
+      inv x3. ss. inv MSG_CLOSED. inv CLOSED1; ss.
+      inv CLOSED2.
+      hexploit Memory.max_full_timemap_spec; try exact PLN; eauto. i.
+      hexploit Memory.max_full_timemap_spec; try exact RLX; eauto. i.
+      econs. econs; ss.
+      * ii. unfold TimeMap.add. condtac; eauto.
+        subst. inv MSG_TS. etrans; [|exact TS].
+        inv MSG_WF. inv WF. apply WF0.
+      * ii. unfold TimeMap.add. condtac; eauto.
+        subst. inv MSG_TS. etrans; [|exact TS]. ss. refl.
+  - exploit (@Memory.split_exists mem1_tgt loc ts1 ts2 ts3 Message.half msg_tgt); eauto; try by econs.
+    i. des. esplits; eauto; econs.
 Qed.
+
+Lemma sim_memory_split_exists
+      loc from_src to_src msg_src mem_src
+      mem1_tgt
+      (CLOSED_SRC: Memory.closed mem_src)
+      (CLOSED_TGT: Memory.closed mem1_tgt)
+      (SIM: sim_memory mem_src mem1_tgt)
+      (GET_SRC: Memory.get loc to_src mem_src = Some (from_src, msg_src)):
+  exists msg_tgt from_tgt to_tgt,
+    <<GET_TGT: Memory.get loc to_tgt mem1_tgt = Some (from_tgt, msg_tgt)>> /\
+    (<<FROM: from_src = from_tgt>> /\
+     <<TO: to_src = to_tgt>>) \/
+    (<<FROM: from_src = from_tgt>> /\
+     <<TO: Time.lt to_src to_tgt>> /\
+     <<SPLIT1: exists msg_tgt' mem2_tgt,
+         Memory.split mem1_tgt loc from_tgt to_src to_tgt msg_tgt' msg_tgt mem2_tgt /\
+         Memory.message_ts msg_tgt' loc to_src /\
+         Memory.closed_message_view msg_tgt' mem2_tgt /\
+         sim_memory mem_src mem2_tgt>>)\/
+    (<<FROM: Time.lt from_tgt from_src>> /\
+     <<TO: to_src = to_tgt>> /\
+     <<SPLIT: exists msg_tgt' mem2_tgt,
+         Memory.split mem1_tgt loc from_tgt from_src to_tgt msg_tgt' msg_tgt mem2_tgt /\
+         Memory.message_ts msg_tgt' loc from_src /\
+         Memory.closed_message_view msg_tgt' mem2_tgt /\
+         sim_memory mem_src mem2_tgt>>) \/
+    (<<FROM: Time.lt from_tgt from_src>> /\
+     <<TO: Time.lt to_src to_tgt>> /\
+     <<SPLIT: exists msg_tgt' msg_tgt'' mem2_tgt mem3_tgt,
+         Memory.split mem1_tgt loc from_tgt from_src to_tgt msg_tgt' msg_tgt mem2_tgt /\
+         Memory.message_ts msg_tgt' loc from_src /\
+         Memory.closed_message_view msg_tgt' mem2_tgt /\
+         Memory.split mem2_tgt loc from_src to_src to_tgt msg_tgt'' msg_tgt mem3_tgt /\
+         Memory.message_ts msg_tgt'' loc to_src /\
+         Memory.closed_message_view msg_tgt'' mem3_tgt /\
+         sim_memory mem_src mem3_tgt>>).
+Proof.
+  dup CLOSED_SRC. inv CLOSED_SRC0.
+  dup CLOSED_TGT. inv CLOSED_TGT0.
+  exploit Memory.get_ts; try exact GET_SRC. i. des.
+  { subst. specialize (INHABITED0 loc).
+    esplits. left. esplits; eauto. }
+  exploit sim_memory_get_inv; try exact GET_SRC; eauto. i. des.
+  exploit Memory.get_ts; try exact GET_TGT. i. des.
+  { subst. inv TO; inv H. inv x0. }
+  exists msg_tgt. inv FROM; inv TO.
+  - esplits. repeat right. splits; eauto.
+    admit.
+  - inv H0. esplits. right. right. left. splits; eauto.
+    admit.
+  - inv H. esplits. right. left. splits; eauto.
+    (* prove that proper split exists *)
+    exploit Memory.split_exists; try exact GET_TGT.
+    { apply x0. }
+    { auto. }
+    { eapply CLOSED0. eauto. }
+    i. des. esplits; eauto. inv SIM. econs.
+    + i. rewrite (@split_covered mem2); eauto.
+    + i. rewrite (@split_covered_half_same mem2); eauto.
+    + i. revert GET. erewrite Memory.split_o; eauto. condtac; ss.
+      * des. subst. i. inv GET.
+  - inv H. inv H0. esplits. left. splits; eauto.
+Admitted.
 
 Lemma sim_memory_add
       mem1_src mem1_tgt msg_src
@@ -366,7 +699,12 @@ Proof.
     econs; i; des; (try by right).
     + left. eapply COVER. eauto.
     + left. eapply COVER. eauto.
-  - i.
+  - i. rewrite add_covered_half; [|eauto]. rewrite (@add_covered_half mem2_tgt); [|eauto].
+    econs; i; des; subst.
+    + left. apply COVER_HALF. auto.
+    + right. inv SIM_MSG. splits; eauto.
+    + left. apply COVER_HALF. auto.
+    + right. inv SIM_MSG. splits; eauto.
   - i. revert GET. erewrite Memory.add_o; eauto. condtac; ss.
     + des. subst. i. inv GET. esplits; eauto.
       erewrite Memory.add_o; eauto. condtac; ss.
@@ -386,6 +724,11 @@ Proof.
   inv SIM. econs.
   - i. rewrite split_covered; [|eauto]. rewrite (@split_covered mem2_tgt); [|eauto].
     apply COVER.
+  - i. rewrite split_covered_half; [|eauto]. rewrite (@split_covered_half mem2_tgt); [|eauto].
+    econs; i; des; subst;
+      try by (left; split; auto; apply COVER_HALF; auto).
+    + right. inv SIM_MSG. split; auto.
+    + right. inv SIM_MSG. split; auto.
   - i. revert GET. erewrite Memory.split_o; eauto. repeat condtac; ss.
     + des. subst. i. inv GET. esplits; eauto.
       erewrite Memory.split_o; eauto. condtac; ss.
@@ -408,9 +751,18 @@ Lemma sim_memory_lower
       (SIM: sim_memory mem1_src mem1_tgt):
   sim_memory mem2_src mem2_tgt.
 Proof.
-  inv SIM. econs.
+  dup SIM. inv SIM0. econs.
   - i. rewrite lower_covered; [|eauto]. rewrite (@lower_covered mem2_tgt); [|eauto].
     apply COVER.
+  - i. rewrite lower_covered_half; [|eauto]. rewrite (@lower_covered_half mem2_tgt); [|eauto].
+    exploit Memory.lower_get0; try exact SRC. i. des.
+    exploit Memory.lower_get0; try exact TGT. i. des.
+    exploit sim_memory_get_from; try exact SIM; eauto. i. des.
+    econs; i; des; subst;
+      try by (left; split; auto; apply COVER_HALF; auto).
+    + admit.
+    + admit.
+    +
   - i. revert GET. erewrite Memory.lower_o; eauto. condtac; ss.
     + des. subst. i. inv GET. esplits; eauto.
       erewrite Memory.lower_o; eauto. condtac; ss.
